Starting proof of soundness optimization ADD_0

optimizations.v
@@ -6,10 +6,55 @@ Require Import List.
 Require Import Coq_EVM.lib.evmModel.
 Require Import Coq_EVM.datatypes.
 Import EVM_Def Concrete Abstract.
+Require Import Coq_EVM.interpreter.
+Import Interpreter SFS.
 Import ListNotations.
 
 
+
 (* Enrique *)
+
+(* ADD(0,X) --> X *)
+Fixpoint optimize_map_add_zero1 (fresh_var: nat) (map: asfs_map): 
+  option asfs_map :=
+match map with
+| [] => None
+| (n, val)::t => if n =? fresh_var then
+                 match val with
+                 | ASFSOp ADD [Val WZero; arg2] =>
+                     Some ((n, ASFSBasicVal arg2)::t)
+                 | _ => None
+                 end
+                 else match optimize_map_add_zero1 fresh_var t with 
+                      | None => None
+                      | Some map' => Some ((n, val)::map')
+                      end
+end.
+
+Definition optimize_func_map (f: nat -> asfs_map -> option asfs_map) 
+  (fresh_var: nat) (s: asfs) : option asfs :=
+match s with
+| ASFSc height maxid stack map => 
+    match f fresh_var map with
+    | None => None
+    | Some map' => Some (ASFSc height maxid stack map')
+    end
+end.
+
+Definition optimize_add_zero1 (fresh_var: nat) (s: asfs) : option asfs :=
+optimize_func_map optimize_map_add_zero1 fresh_var s.
+
+Definition coherent_opm (ops: opm) : Prop :=
+True.
+
+
+Theorem optimize_add_zero1_safe: forall (a1 a2: asfs) (fresh_var: nat)
+  (s: concrete_stack) (ops: opm),
+optimize_add_zero1 fresh_var a1 = Some a2 ->
+eval_asfs s a1 ops = eval_asfs s a2 ops.
+Proof. 
+Admitted.
+
 
 
 
